\section{Příklad 2}


\textbf{Zadání:} Určete všechna $c \in \mathbb{R}$ tak, aby:
\begin{displaymath}
\begin{vmatrix}
c+3 & -1 & -1\\
5 & 3 & c+3\\
-1 & c+3 & c+3\\
\end{vmatrix}
= 0.
\end{displaymath}
\par\noindent\rule{\textwidth}{0.4pt}

\textbf{Krok 1:} Určíme determinant soustavy.
\begin{displaymath}
|A|=
\begin{vmatrix}
c+3 & -1 & -1\\
5 & 3 & c+3\\
-1 & c+3 & c+3\\
\end{vmatrix}
\end{displaymath}
\begin{displaymath}
\begin{matrix}
|A| = 3(c+3)^2-5(c+3)+(c+3)-(3+(c+3)^3-5(c+3)) =\\
= 3(c+3)^2-5(c+3)+(c+3)-3-(c+3)^3+5(c+3)) =\\
= -(c+3)^3+3(c+3)^2+(c+3)-3=\\
= -(c^3+9c^2+27c+27)+3(c^2+6c+9)+c=\\
= -c^3-9c^2-27c-27)+3c^2+18c+27+c=\\
= -c^3-6c^2-8c=\\
=-c(c^2+6c+8)=\\
=-c(c+4)(c+2)\\
\end{matrix}
\end{displaymath}

\textbf{Krok 2:} Určíme, kdy je determinant roven 0.
\begin{displaymath}
\begin{matrix}
-c(c+4)(c+2) = 0\\
\end{matrix}
\end{displaymath}
\begin{displaymath}
\begin{matrix}
-c = 0 & \implies & c = 0 \\
c+4=0 & \implies & c=-4\\
c+2=0 & \implies & c=-2 
\end{matrix}
\end{displaymath}

\textbf{Řešení:}
\begin{displaymath}
|A|=0 \Longleftrightarrow c \in \{0, -2, -4\}
\end{displaymath}
